GDS_Testing.v
@@ -7,7 +7,7 @@ Open Scope expr.
 
 
 Ltac inv H := inversion H; subst; clear H.
-Ltac prover := try repeat eexists; try repeat split; try reflexivity.
+Ltac prover := try repeat eexists; try repeat split; cbv; try reflexivity.
 
 Ltac general_match := match goal with
     | [|- _ -> _]  => intros
@@ -143,9 +143,11 @@ Qed.
 
 (*STARTING DUALS*)
 
+Definition defaultVal: valuation * valuation := ($0 $+ ("current", varAss 1), $0).
+
 Theorem runStmtDualVar :    
     exists vg2 vl2, 
-    runStmtDual 10 ($0 $+ ("current", varAss 1), $0) $0 
+    runStmtDual 10 defaultVal $0 
     ((var "a" := Const 2) ;; (var "b" := Const 3) ;; 
     (var "ret" := ((Var "a") + (Var "b"))) ;; skip) = Some (vg2, vl2)
     /\ (vl2 $? "ret" = Some (varAss 5)).
@@ -156,7 +158,7 @@ Qed.
 
 Theorem runStmtDualIf :
     exists vg2 vl2, 
-    (runStmtDual 4 ($0 $+ ("current", varAss 1), $0) $0 
+    (runStmtDual 4 defaultVal $0 
     ((( (var "a" := Const 2 ;; var "b" := Const 3) ;; 
     when ((Var "b") - (Var "a")) 
     then (var "ret" := Const 10) 
@@ -170,7 +172,7 @@ Qed.
 
 Theorem runStmtDualWhile :
     exists vg2 vl2, 
-    (runStmtDual 6 ($0 $+ ("current", varAss 1), $0) $0 
+    (runStmtDual 6 defaultVal $0 
     ((((var "a" := Const 2 ;; while (Var "a") loop ("a" <- Var "a" - Const 1) done) ;; 
     var "ret" := Var "a" + Const 5) ;; skip))) = Some (vg2, vl2)
     /\ (vl2 $? "ret" = Some (varAss 5)).
@@ -190,9 +192,137 @@ Definition dB1 := (topVar "a" := Const 3 ;;; topVar "ret" := Const 0 ;;;
 
 
 Theorem RunDualProgsNoOverlap :
-    exists vg2, (runDual 15 ($0 $+ ("current", varAss 1), $0) dA1 dB1
+    exists vg2, (runDual 15 defaultVal dA1 dB1
     ) = Some vg2 
     /\ (fst vg2 $? "ret" = Some (varAss 10)) /\ (snd vg2 $? "ret" = Some (varAss 4)).
 Proof.
     prover.
+Qed.
+
+
+Definition dA2 := (topVar "ret" := Const 3 ;;;
+    readyDecl (awaitStmt "sigB" ;; "ret" <- Const 10) ;;; 
+    EndDecl).
+
+Definition dB2 := readyDecl (emitSignalStmt "sigB" None nil) ;;; EndDecl.
+
+Theorem RunDualSimpleAwait :
+    exists vg2, (runDual 10 defaultVal dA2 dB2
+    ) = Some vg2 
+    /\ (fst vg2 $? "ret" = Some (varAss 10)).
+Proof.
+    prover.
+Qed.
+
+
+Definition dA3 := (topVar "ret" := Const 3 ;;; 
+    methodDecl "func" ("a" :: nil) None ("ret" <- Var "a") ;;;
+    readyDecl (awaitStmt "sigB" ;; "ret" <- Const 10) ;;; 
+    EndDecl).
+
+Definition dB3 := readyDecl (emitSignalStmt "sigB" (Some ("func", 1)) (Const 8 :: nil)) ;;; EndDecl.
+
+
+(*Context switch for callback and waiting*)
+Theorem RunDualEmitSignalCallbackAndAwait1 :
+    exists vg2, (runDual 10 defaultVal dA2 dB2
+    ) = Some vg2 
+    /\ (fst vg2 $? "ret" = Some (varAss 10)).
+Proof.
+    prover.
+Qed.
+
+
+Definition dA3' := (topVar "ret" := Const 3 ;;; 
+    methodDecl "func" ("a" :: nil) None ("ret" <- Var "a") ;;;
+    EndDecl).
+
+Definition dB3' := (topVar "ret" := Const 0 ;;; 
+    readyDecl (awaitStmt "sigB" ;; "ret" <- Const 10) ;;; 
+    processDecl (emitSignalStmt "sigB" (Some ("func", 1)) (Const 8 :: nil)) ;;; 
+    EndDecl).
+
+(*Context switch for callback but not await*)
+Theorem RunDualEmitSignalCallbackAndAwait2 :
+    exists vg2, (runDual 10 defaultVal dA3' dB3'
+    ) = Some vg2 
+    /\ (fst vg2 $? "ret" = Some (varAss 8)) /\ (snd vg2 $? "ret" = Some (varAss 10)).
+Proof.
+    eexists; repeat split; cbv; reflexivity.
+Qed.
+
+Definition dA3'' := (topVar "ret" := Const 3 ;;; 
+    methodDecl "func" ("a" :: nil) None ("ret" <- Var "a") ;;;
+    processDecl (emitSignalStmt "sigA" (Some ("func", 1)) (Const 8 :: nil)) ;;; 
+    EndDecl).
+
+Definition dB3'' := (topVar "ret" := Const 0 ;;; 
+    readyDecl (awaitStmt "sigA" ;; "ret" <- Const 10) ;;; 
+    EndDecl).
+
+(*Context switch for await but not callback*)
+Theorem RunDualEmitSignalCallbackAndAwait3 :
+    exists vg2, (runDual 10 defaultVal dA3'' dB3''
+    ) = Some vg2 
+    /\ (fst vg2 $? "ret" = Some (varAss 8)) /\ (snd vg2 $? "ret" = Some (varAss 10)).
+Proof.
+    eexists; repeat split; cbv; reflexivity.
+Qed.
+
+
+
+(*Next: One program awaits the other, ret should be 10 if the signal is received after the first program has done two loops*)
+
+Definition dA4 := (topVar "a" := Const 0 ;;; topVar "ret" := Const 3 ;;;
+    readyDecl (awaitStmt "sigB" ;; "ret" <- Const 10) ;;; 
+    processDecl( "a" <- Var "a" + Const 1 ;; 
+        when (Var "a" == Const 2)
+        then ("ret" <- Const 5)
+        else (skip)
+        done);;; EndDecl).
+
+Definition dB4 := (topVar "a" := Const 0 ;;;
+    processDecl( "a" <- Var "a" + Const 1 ;; 
+        when (Var "a" == Const 4)
+        then (emitSignalStmt "sigB" None nil)
+        else (skip)
+        done);;; EndDecl).
+
+
+(*When running alone, the first program does set ret to 5*)
+Lemma RunMonoAwaitForever :
+    exists vg2, (run 20 $0 dA4) = Some vg2 /\ vg2 $? "ret" = Some (varAss 5).
+Proof.
+    prover.
+Qed.
+
+(*Very strong theorem*)
+Theorem RunDualProgsAwait :
+    exists vg2, (runDual 14 defaultVal dA4 dB4
+    ) = Some vg2 
+    /\ (fst vg2 $? "ret" = Some (varAss 10)).
+Proof.
+    eexists; split; cbv; reflexivity.
+Qed.
+
+
+(*Now having B wait for A to check the symmetry*)
+
+Definition dA5 := (topVar "a" := Const 0 ;;;
+    processDecl( "a" <- Var "a" + Const 1 ;; 
+        when (Var "a" == Const 3)
+        then (emitSignalStmt "sigA" None nil)
+        else (skip)
+        done);;; EndDecl).
+
+Definition dB5 := (topVar "a" := Const 0 ;;; topVar "ret" := Const 3 ;;;
+    readyDecl (awaitStmt "sigA" ;; "ret" <- Const 10) ;;; 
+    processDecl( "a" <- Var "a" + Const 1) ;;; EndDecl).
+
+Theorem RunDualProgsAwaitSymmetric :
+    exists vg2, (runDual 14 defaultVal dA5 dB5
+    ) = Some vg2 
+    /\ (snd vg2 $? "ret" = Some (varAss 10)).
+Proof.
+    eexists; split; cbv; reflexivity.
 Qed.
